src/Lustre/LCausality.v
@@ -1,0 +1,80 @@
+From Coq Require Import List.
+Import List.ListNotations.
+Open Scope list_scope.
+From Coq Require Import Permutation.
+
+From Velus Require Import Common.
+From Velus Require Import Operators.
+From Velus Require Import Clocks.
+
+From Velus Require Import Lustre.LSyntax.
+
+(** * Lustre causality *)
+
+(**
+  Causality judgement over a Lustre program
+  *)
+
+Module Type LCAUSALITY
+       (Import Ids : IDS)
+       (Import Op : OPERATORS)
+       (Import Syn : LSYNTAX Ids Op).
+
+  Inductive Is_free_left (x : ident) : exp -> Prop :=
+  | IFLvar : forall a,
+      Is_free_left x (Evar x a)
+  | IFLunop : forall op e a,
+      Is_free_left x e ->
+      Is_free_left x (Eunop op e a)
+  | IFLbinop : forall op e1 e2 a,
+      Is_free_left x e1
+      \/ Is_free_left x e2 ->
+      Is_free_left x (Ebinop op e1 e2 a)
+  | IFLfby : forall e0s es a,
+      Exists (Is_free_left x) e0s ->
+      Is_free_left x (Efby e0s es a)
+  | IFLwhen : forall es y b a,
+      x = y
+      \/ Exists (Is_free_left x) es ->
+      Is_free_left x (Ewhen es y b a)
+  | IFLmerge : forall ets efs y a,
+      x = y
+      \/ Exists (Is_free_left x) ets
+      \/ Exists (Is_free_left x) efs ->
+      Is_free_left x (Emerge y ets efs a)
+  | IFLite : forall e ets efs a,
+      Is_free_left x e
+      \/ Exists (Is_free_left x) ets
+      \/ Exists (Is_free_left x) efs ->
+      Is_free_left x (Eite e ets efs a)
+  | IFLapp : forall f es a,
+      Exists (Is_free_left x) es ->
+      Is_free_left x (Eapp f es None a)
+  | IFLreset : forall f es r a,
+      Exists (Is_free_left x) (r :: es) ->
+      Is_free_left x (Eapp f es (Some r) a).
+
+  Inductive Is_causal (inputs : list ident) : list equation -> Prop :=
+  | ICnil:
+      Is_causal inputs []
+  | ICcons: forall eq eqs,
+      Is_causal inputs eqs ->
+      (forall x, Exists (Is_free_left x) (snd eq) ->
+            In x (vars_defined eqs) \/ In x inputs) ->
+      Is_causal inputs (eq :: eqs).
+  Hint Constructors Is_causal.
+
+  (* TODO: link with check_graph_spec *)
+  Definition node_causal (n : node) :=
+    exists eqs, Permutation (n_eqs n) eqs
+           /\ Is_causal (map fst (n_in n)) eqs.
+
+End LCAUSALITY.
+
+Module LCausality
+       (Ids  : IDS)
+       (Op   : OPERATORS)
+       (Syn  : LSYNTAX Ids Op)
+       <: LCAUSALITY Ids Op Syn.
+  Include LCAUSALITY Ids Op Syn.
+End LCausality.
