src/Lustre/Lustre.v
@@ -4,8 +4,9 @@ From Velus Require Import CoindStreams.
 From Velus Require Export Lustre.LSyntax.
 From Velus Require Export Lustre.LClocking.
 From Velus Require Export Lustre.LTyping.
-From Velus Require Export Lustre.LSemantics.
 From Velus Require Export Lustre.LOrdered.
+From Velus Require Export Lustre.LCausality.
+From Velus Require Export Lustre.LSemantics.
 From Velus Require Export Lustre.LClockSemantics.
 From Velus Require Export Lustre.Normalization.LNormalization.
 
@@ -21,6 +22,7 @@ Module Type LUSTRE
   Declare Module Export Typ: LTYPING    Ids Op       Syn.
   Declare Module Export Clo: LCLOCKING  Ids Op       Syn.
   Declare Module Export Lord: LORDERED  Ids Op       Syn.
+  Declare Module Export Lcau: LCAUSALITY Ids Op       Syn.
   Declare Module Export Sem: LSEMANTICS Ids Op OpAux Syn Lord Str.
   Declare Module Export ClockSem : LCLOCKSEMANTICS Ids Op OpAux Syn Typ Clo Lord Str Sem.
   Declare Module Export Norm: LNORMALIZATION Ids Op OpAux Str Syn Typ Clo Lord Sem.
@@ -36,6 +38,7 @@ Module LustreFun
   Module Export Typ := LTypingFun     Ids Op       Syn.
   Module Export Clo := LClockingFun   Ids Op       Syn.
   Module Export Lord:= LOrderedFun    Ids Op       Syn.
+  Module Export Lcau:= LCausality     Ids Op       Syn.
   Module Export Sem := LSemanticsFun  Ids Op OpAux Syn Lord Str.
   Module Export ClockSem := LClockSemanticsFun Ids Op OpAux Syn Typ Clo Lord Str Sem.
   Module Export Norm := LNormalizationFun Ids Op OpAux Str Syn Typ Clo Lord Sem.
